LeanSubst/Types/List.lean
@@ -7,7 +7,7 @@ universe u1 u2 u3
 variable {S : Type u1} {T T1 T2 : Type u2} {U : Type u3}
 variable {V : List (Type u2)}
 
-def List.rmap [RenMap S V] (r : List.Tuple Ren V) : List S -> List S
+def List.rmap [RenMap S V] (r : RenVec V) : List S -> List S
 | [] => []
 | .cons x xs => x⟨r,⟩ :: rmap r xs
 
@@ -15,11 +15,11 @@ instance [RenMap S V] : RenMap (List S) V where
   rmap := List.rmap
 
 @[simp, grind =]
-theorem List.rmap_nil [RenMap S V] {r : List.Tuple Ren V} : (@List.nil S)⟨r,⟩ = [] := by
+theorem List.rmap_nil [RenMap S V] {r : RenVec V} : (@List.nil S)⟨r,⟩ = [] := by
   simp [RenMap.rmap, List.rmap]
 
 @[simp, grind =]
-theorem List.rmap_cons [RenMap S V] {x} {xs : List S} {r : List.Tuple Ren V} : (x::xs)⟨r,⟩ = x⟨r,⟩::xs⟨r,⟩ := by
+theorem List.rmap_cons [RenMap S V] {x} {xs : List S} {r : RenVec V} : (x::xs)⟨r,⟩ = x⟨r,⟩::xs⟨r,⟩ := by
   simp [RenMap.rmap, List.rmap]
 
 instance [RenMap S V] [RenMapId S V] : RenMapId (List S) V where
@@ -29,11 +29,11 @@ instance [RenMap S V] [RenMapCompose S V] : RenMapCompose (List S) V where
   apply_compose := by intro s σ τ; induction s <;> simp [*]
 
 @[simp]
-theorem List.rmap_append [RenMap S V] {xs ys : List S} {r : List.Tuple Ren V}
+theorem List.rmap_append [RenMap S V] {xs ys : List S} {r : RenVec V}
   : (xs ++ ys)⟨r,⟩ = xs⟨r,⟩ ++ ys⟨r,⟩
 := by induction xs generalizing ys <;> simp [*]
 
-def List.smap [SubstMap S V] (σ : List.Tuple Subst V) : List S -> List S
+def List.smap [SubstMap S V] (σ : SubstVec V) : List S -> List S
 | [] => []
 | .cons x xs => x[σ,] :: smap σ xs
 
@@ -41,11 +41,11 @@ instance [SubstMap S V] : SubstMap (List S) V where
   smap := List.smap
 
 @[simp, grind =]
-theorem List.smap_none [SubstMap S V] {σ : List.Tuple Subst V} : (@List.nil S)[σ,] = [] := by
+theorem List.smap_none [SubstMap S V] {σ : SubstVec V} : (@List.nil S)[σ,] = [] := by
   simp [SubstMap.smap, List.smap]
 
 @[simp, grind =]
-theorem List.smap_some [SubstMap S V] {x} {xs : List S} {σ : List.Tuple Subst V} : (x::xs)[σ,] = x[σ,]::xs[σ,]
+theorem List.smap_some [SubstMap S V] {x} {xs : List S} {σ : SubstVec V} : (x::xs)[σ,] = x[σ,]::xs[σ,]
 := by simp [SubstMap.smap, List.smap]
 
 instance [RenMap S V] [SubstMap S V] [SubstMapId S V] : SubstMapId (List S) V where
